Fix executable version of analysis

SimAsm/SimAsm_Inter_Exec.thy
@@ -1,433 +1,462 @@
 theory SimAsm_Inter_Exec
-  imports SimAsm_Inter "HOL-Library.While_Combinator" "HOL-Eisbach.Eisbach"
+  imports "HOL-Library.FSet" "SimAsm_Inter" "HOL-Library.While_Combinator"
 begin
 
 text \<open>
-Theorems to demonstrate termination of the SimAsm_Inter analysis 
-and demonstrate its conversion to executable definitions.
+This theory file describes the executable interference pairs analysis
+and relates it to the abstract.
 \<close>
 
-section \<open>Termination Proof\<close>
+type_synonym ('v,'g,'r,'a) enumi = "('v,'g,'r,'a) pred \<times> ('v,'g,'r) op \<times> ('v,'g,'r,'a) auxfn"
+type_synonym ('v,'g,'r,'a) enuml = "('v,'g,'r,'a) enumi list"
 
-abbreviation vars
-  where "vars p \<equiv> (rds p |\<union>| wrs p)"
+text \<open>A data point, extends an instruction with reordering information\<close>
+record ('g,'r) point =
+  id :: nat
+  wrs :: "('g,'r) var fset"
+  rds :: "('g,'r) var fset"
+  bar :: bool
+  esc :: "('g,'r) var fset"
+  pairs :: "(nat \<times> ('g,'r) var fset) fset"
 
-definition nmax
-  where "nmax V \<equiv> if V = {||} then 0 else fMax V"
+definition hasGlobal\<^sub>e
+  where "hasGlobal\<^sub>e S \<equiv> \<exists>e. Glb e |\<in>| S"
 
-definition pmax
-  where "pmax p \<equiv> max (id p) (nmax (pairs p))"
+fun hasGlobalL
+  where "hasGlobalL (Glb x#a) = True" | 
+        "hasGlobalL [] = False" |
+        "hasGlobalL (b#a) = hasGlobalL a"
 
-definition Pmax
-  where "Pmax P \<equiv> if P = {} then 0 else Max (pmax ` P)"
+text \<open>Substitute a variable for an expression\<close>
+fun subst :: "('v,'g,'r) exp \<Rightarrow> ('g,'r) var \<Rightarrow> ('v,'g,'r) exp \<Rightarrow> ('v,'g,'r) exp"
+  where
+    "subst (Var r) r' e = (if r = r' then e else Var r)" |
+    "subst (Exp f rs) r e = (Exp f (map (\<lambda>x. subst x r e) rs))" |
+    "subst e _ _ = e"
 
-definition varsL
-  where "varsL l = Sup ((\<lambda>p. fwr p |\<union>| frd p) ` (set l))"
+text \<open>The syntactic dependencies of an expression\<close>
+fun ldeps :: "('v,'g,'r) exp \<Rightarrow> ('g,'r) var list"
+  where 
+    "ldeps (Var r) = [r]" |
+    "ldeps (Exp _ rs) = List.bind rs ldeps" |
+    "ldeps _ = []"
 
-definition all_points
-  where "all_points vs i \<equiv> {p. vars p |\<subseteq>| vs \<and> id p \<le> i \<and> nmax (pairs p) \<le> i}"
+fun ldeps\<^sub>B :: "('v,'g,'r) bexp \<Rightarrow> ('g,'r) var list"
+  where 
+    "ldeps\<^sub>B (Neg e) = ldeps\<^sub>B e" |
+    "ldeps\<^sub>B (Exp\<^sub>B _ rs) = List.bind rs ldeps"
 
-lemma finite_all_points [intro]:
-  "finite (all_points vs i :: ('a, 'b) point set)"
-proof -
-  let ?f = "\<lambda>d w r b p. \<lparr>id = d, wrs = w, rds = r, bar = b, pairs = p\<rparr>"
-  have a: "finite {w. w |\<subseteq>| vs}"
-  proof -
-    have "finite (Abs_fset ` {w. w \<subseteq> fset vs})" by simp
-    moreover have "{w. w |\<subseteq>| vs} \<subseteq> Abs_fset ` {w. w \<subseteq> fset vs}"
-      by (auto simp: fset_inverse less_eq_fset.rep_eq rev_image_eqI)
-    ultimately show ?thesis by (meson finite_subset)
-  qed
-  have b: "finite {p. nmax p \<le> i}"
-  proof -
-    have "finite {p. p \<subseteq> {j. j \<le> i}}" by blast
-    hence f: "finite {p. finite p \<and> Max p \<le> i}"
-      by (rule rev_finite_subset; insert Max.boundedE; auto)
-    hence "finite (insert {||} (Abs_fset ` {p. finite p \<and> Max p \<le> i}))" 
-      by blast
-    thus ?thesis
-      apply (rule rev_finite_subset)
-      apply (auto simp: nmax_def)
-      by (metis (no_types, lifting) fMax.F.rep_eq finite_fset fset_inverse image_iff mem_Collect_eq)
-  qed
-  have c: "finite {?f d w r b p | d w r b p. w |\<subseteq>| vs \<and> r |\<subseteq>| vs \<and> d \<le> i \<and> nmax p \<le> i}"
-    using a b finite_subset[where 
-        A="{?f d w r b p | d w r b p. w |\<subseteq>| vs \<and> r |\<subseteq>| vs \<and> d \<le> i \<and> nmax p \<le> i}" and 
-        B="\<Union>d \<in> {d. d \<le> i}. \<Union>w \<in> {w. w |\<subseteq>| vs}. \<Union>r \<in> {r. r |\<subseteq>| vs}. \<Union>b \<in> UNIV. \<Union>p \<in> {p. nmax p \<le> i}. {?f d w r b p}"]
-    by fastforce
-  have d: "all_points vs i \<subseteq> {?f d w r b p | d w r b p. w |\<subseteq>| vs \<and> r |\<subseteq>| vs \<and> d \<le> i \<and> nmax p \<le> i}"
-    unfolding all_points_def
-    by auto (metis point.cases point.select_convs(1,2,3,5))
-  show "finite (all_points vs i :: ('a, 'b) point set)"
-    using finite_subset[OF d c] .
-qed
+definition fdeps 
+  where "fdeps a = fset_of_list (ldeps a)"
 
-lemma all_points_rel:
-  "P |\<subseteq>| P' \<Longrightarrow> i \<le> i' \<Longrightarrow> all_points P i \<subseteq> all_points P' i'"
-  unfolding all_points_def by auto
+definition fdeps\<^sub>B
+  where "fdeps\<^sub>B a = fset_of_list (ldeps\<^sub>B a)"
 
-lemma max_fg:
-  assumes "finite P" "\<forall>p. f p \<le> g p"
-  shows "Max (f ` P) \<le> Max (g ` P)"
-  using assms 
-  by (smt Max_ge_iff Max_in finite_imageI imageE image_eqI image_is_empty order_refl) 
+text \<open>Variables written by an operation\<close>
+fun fwr :: "('v,'g,'r) op \<Rightarrow> ('g,'r) var fset"
+  where 
+    "fwr (assign y _) = {|y|}" |
+    "fwr _ = {||}"
 
-lemma Max_max :
-  "finite V \<Longrightarrow> Max ((\<lambda>p. max (f p) (g p)) ` V) = max (Max (f ` V)) (Max (g ` V))" (is "finite V \<Longrightarrow> ?L = ?R")
-proof -
-  assume a: "finite V"
-  have "?L \<ge> ?R"
-  proof -
-    have "Max (f ` V) \<le> ?L" using a by (rule max_fg) auto
-    moreover have "Max (g ` V) \<le> ?L" using a by (rule max_fg) auto
-    ultimately show "?L \<ge> ?R" by auto
-  qed
-  moreover have "?R \<ge> ?L"
-  proof (cases "Max (f ` V) \<ge> Max (g ` V)")
-    case True
-    hence "max (Max (f ` V)) (Max (g ` V)) = Max (f ` V)" using max_absorb1 by blast
-    moreover have "(MAX p\<in>V. max (f p) (g p)) \<le> (Max (f ` V))" using a
-      by (smt Max_ge Max_in calculation dual_order.trans finite_imageI image_iff image_is_empty max.absorb_iff1 max_def)
-    ultimately show ?thesis by auto
-  next
-    case False
-    hence "max (Max (f ` V)) (Max (g ` V)) = Max (g ` V)" using linear max_absorb2 by blast
-    moreover have "(MAX p\<in>V. max (f p) (g p)) \<le> (Max (g ` V))" using a
-      by (smt Max_ge Max_in calculation dual_order.trans finite_imageI image_iff image_is_empty max.absorb_iff1 max_def)
-    ultimately show ?thesis by auto
-  qed
-  ultimately show ?thesis using eq_iff by blast
-qed
+fun lfwr :: "('v,'g,'r) op \<Rightarrow> ('g,'r) var fset"
+  where 
+    "lfwr (assign (Reg y) _) = {|Reg y|}" |
+    "lfwr _ = {||}"
 
-lemma set_all_points_bound:
-  "finite P \<Longrightarrow> P \<subseteq> all_points (Sup (vars ` P)) (Pmax P)"
-  unfolding all_points_def
-proof (clarsimp, intro conjI, goal_cases)
-  case (1 x)
-  hence "vars x |\<subseteq>| Sup (vars ` P)" 
-    by (meson finite_imageI image_iff le_cSup_finite)
-  then show ?case by blast
-next
-  case (2 x)
-  hence "vars x |\<subseteq>| Sup (vars ` P)" 
-    by (meson finite_imageI image_iff le_cSup_finite)
-  then show ?case by blast
-next
-  case (3 x)
-  hence "id x \<le> (MAX p\<in>P. id p)" by simp
-  also have "... \<le> (MAX p\<in>P. max (id p) (nmax (pairs p)))"
-    apply (rule max_fg)
-    using 3 by auto
-  also have "... \<le> Pmax P" using 3 by (auto simp: Pmax_def pmax_def)
-  finally show ?case .
-next
-  case (4 x)
-  hence "nmax (pairs x) \<le> (MAX p\<in>P. nmax (pairs p))" by simp
-  also have "... \<le> (MAX p\<in>P. max (id p) (nmax (pairs p)))"
-    apply (rule max_fg)
-    using 4 by auto
-  also have "... \<le> Pmax P" using 4 by (auto simp: Pmax_def pmax_def)
-  finally show ?case .
-qed
+text \<open>Variables read by an operation\<close>
+fun frd :: "('v,'g,'r) op \<Rightarrow> ('g,'r) var fset"
+  where
+    "frd (assign _ e) = fdeps e" |
+    "frd (cmp b) = fdeps\<^sub>B b" |
+    "frd _ = {||}"
 
-lemma set_all_points_bound':
-  "finite P \<Longrightarrow> P \<subseteq> all_points (varsL l |\<union>| Sup (vars ` P)) (max (length l) (Pmax P))"
-  using set_all_points_bound all_points_rel
-  by (metis (mono_tags, lifting) subset_trans sup_ge2 sup_max)
+text \<open>Conditions under which a point is ordered after an instruction\<close>
+fun ord\<^sub>e
+  where
+    "ord\<^sub>e nop p = (bar p)" |
+    "ord\<^sub>e (cmp b) p = (bar p \<or> hasGlobal\<^sub>e (wrs p) \<or> hasGlobal\<^sub>e (fdeps\<^sub>B b |\<inter>| rds p))" |
+    "ord\<^sub>e (assign v e) p = 
+      (bar p \<or> 
+        hasGlobal\<^sub>e (fdeps e |\<inter>| (rds p |\<union>| wrs p)) \<or> 
+        (case v of Glb g \<Rightarrow> Glb g |\<in>| wrs p | _ \<Rightarrow> False) \<or> 
+        (hasGlobal\<^sub>e (fdeps e) \<and> v |\<in>| rds p))" |
+    "ord\<^sub>e full_fence _ = True"
 
-lemma fsubset_sup:
-  "\<forall>j \<in> Y. f j |\<subseteq>| X \<Longrightarrow> Sup (f ` Y) |\<subseteq>| X"
-proof -
-  assume "\<forall>j \<in> Y. f j |\<subseteq>| X"
-  hence "\<forall>j \<in> Y. fset (f j) \<subseteq> fset X" by (simp add: less_eq_fset.rep_eq)
-  hence "Sup ((fset o f) ` Y) \<subseteq> fset X" by auto
-  thus "Sup (f ` Y) |\<subseteq>| X" 
-    by (simp add: Sup_fset.rep_eq less_eq_fset.rep_eq) 
-qed
+text \<open>Strengthen a point based on a strictly earlier instruction\<close>
+definition stren :: "('v,'g,'r) op \<Rightarrow> ('g,'r) point \<Rightarrow> ('g,'r) point"
+  where
+    "stren a p = p\<lparr> wrs := wrs p |\<union>| fwr a, 
+                    rds := rds p |-| lfwr a |\<union>| frd a, 
+                    bar := bar p \<or> barriers a \<rparr>"
 
-lemma all_points_sub:
-  assumes "Y \<subseteq> (all_points vs i :: ('a, 'b) point set)"
-  shows "all_points (Sup (vars ` Y)) (Pmax Y) \<subseteq> all_points vs i"
-proof (rule all_points_rel)
-  have "\<forall>j \<in> pmax ` Y. j \<le> i"
-    using assms by (auto simp: all_points_def pmax_def)
-  moreover have "finite Y" using finite_subset[OF assms finite_all_points] .
-  ultimately show "Pmax Y \<le> i" unfolding Pmax_def by auto
-next
-  have "\<forall>j \<in> Y. vars j |\<subseteq>| vs" using assms by (auto simp: all_points_def)
-  thus "Sup (vars ` Y) |\<subseteq>| vs" using fsubset_sup by fast
-qed
+text \<open>Weaken a point based on a reorderable instruction\<close>
+definition wken :: "nat \<Rightarrow> ('v,'g,'r) op \<Rightarrow> ('g,'r) point \<Rightarrow> ('g,'r) point"
+  where
+    "wken n \<alpha> p = p\<lparr> rds := rds p - fwr \<alpha> |\<union>| 
+                            (if fwr \<alpha> |\<inter>| rds p \<noteq> {||} then frd \<alpha> else {||}), 
+                     esc := esc p |\<union>| fwr \<alpha>,
+                     pairs := pairs p |\<union>| {|(n, esc p)|} \<rparr>"
 
-lemma all_points_rel_rev:
-  "all_points v i \<subseteq> (all_points v' i' :: ('a, 'b) point set) \<Longrightarrow> (v |\<subseteq>| v' \<and> i \<le> i')"
-proof (rule ccontr)
-  assume s: "all_points v i \<subseteq> (all_points v' i' :: ('a, 'b) point set)" "\<not> (v |\<subseteq>| v' \<and> i \<le> i')"
-  hence "\<not> v |\<subseteq>| v' \<or> i > i'" by auto
-  hence "\<lparr>id = i, wrs = v, rds = v, bar = True, pairs = {||}\<rparr> \<notin> all_points v' i'"
-    by (auto simp: all_points_def nmax_def)
-  moreover have "\<lparr>id = i, wrs = v, rds = v, bar = True, pairs = {||}\<rparr> \<in> all_points v i"
-    by (auto simp: all_points_def nmax_def)
- ultimately show "False" using s(1) by auto
-qed
+text \<open>Convert an instruction into a point\<close>
+abbreviation gen :: "nat \<Rightarrow> ('v,'g,'r) op \<Rightarrow> ('g,'r) point"
+  where
+    "gen n a \<equiv> \<lparr> id = n, wrs = fwr a, rds = frd a, bar = barriers a, esc = {||}, pairs = {||} \<rparr>"
 
-lemma all_points_const:
-  assumes "all_points v i \<subseteq> (all_points v' i' :: ('a, 'b) point set)"
-  shows "all_points (c |\<union>| v) (max ic i) \<subseteq> all_points (c |\<union>| v') (max ic i')"
-proof -
-  have "v |\<subseteq>| v' \<and> i \<le> i'" using all_points_rel_rev[OF assms] by auto
-  thus ?thesis by (intro all_points_rel) auto
-qed
+text \<open>Process a new instruction against one point\<close>
+definition proc1 :: "nat \<Rightarrow> ('v,'g,'r) op \<Rightarrow> (_,_) point \<Rightarrow> (_,_) point set"
+  where "proc1 n \<alpha> p \<equiv> if ord\<^sub>e \<alpha> p then {stren \<alpha> p} else {stren \<alpha> p, wken n \<alpha> p}"
+
+text \<open>Process a new instruction against a set of points\<close>
+definition rif\<^sub>i :: "nat \<Rightarrow> ('v,'g,'r) op \<Rightarrow> ('g,'r) point set \<Rightarrow> ('g,'r) point set"
+  where 
+    "rif\<^sub>i n a P \<equiv> { gen n a } \<union> \<Union> (proc1 n a ` P)"
+
+text \<open>Process a full program\<close>
+fun rif :: "(nat, nat) com \<Rightarrow> ('v,'g,'r) op list \<Rightarrow> ('g,'r) point set \<Rightarrow> ('g,'r) point set"
+  where 
+    "rif (Basic a) l P = (rif\<^sub>i (tag a) (l ! (tag a)) P)" |
+    "rif (Choice c\<^sub>1 c\<^sub>2) l P = (rif c\<^sub>1 l P \<union> rif c\<^sub>2 l P)" |
+    "rif (Loop c) l P = lfp (\<lambda>Y. (P \<union> rif c l Y))" |
+    "rif (c\<^sub>1 ;; c\<^sub>2) l P = rif c\<^sub>1 l (rif c\<^sub>2 l P)" |
+    "rif _ _ P = P"
+declare rif.simps(3)[simp del]
+
+fun enum :: "('v,'g,'r,'a) lang \<Rightarrow> ('v,'g,'r,'a) enuml \<Rightarrow> (nat, nat) com \<times> ('v,'g,'r,'a) enuml"
+  where
+    "enum Skip l = (com.Nil,l)" |
+    "enum (Op v a f) l = (Basic (length l,{},{}),l@[(v,a,f)])" |
+    "enum (Seq c\<^sub>1 c\<^sub>2) l = 
+      (case enum c\<^sub>2 l of (n\<^sub>2,l) \<Rightarrow> (case enum c\<^sub>1 l of (n\<^sub>1,l) \<Rightarrow> (com.Seq n\<^sub>1 n\<^sub>2,l)))" |
+    "enum (If b c\<^sub>1 c\<^sub>2) l = 
+      (case enum c\<^sub>2 l of (n\<^sub>2,l) \<Rightarrow> case enum c\<^sub>1 l of (n\<^sub>1,l) \<Rightarrow> 
+        (Choice (com.Seq (Basic (length l,{},{})) n\<^sub>1) (com.Seq (Basic (Suc (length l),{},{})) n\<^sub>2),
+          l@[(UNIV,cmp b,state_rec.more),(UNIV,cmp (Neg b),state_rec.more)]))" |
+    "enum (While b I c) l = 
+      (case enum c l of (n,l) \<Rightarrow> 
+        (com.Seq ((com.Seq (Basic (length l,{},{})) n)*) (Basic (Suc (length l),{},{})),
+          l@[(UNIV,cmp b,state_rec.more),(UNIV,cmp (Neg b),state_rec.more)]))" |
+    "enum (DoWhile I c b) l = 
+      (case enum c l of (n,l) \<Rightarrow> 
+        ((n ;; Basic (length l,{},{}))* ;; n ;; Basic (Suc (length l),{},{}), 
+          l@[(UNIV,cmp b,state_rec.more),(UNIV,cmp (Neg b),state_rec.more)]))" 
+
+subsection \<open>Refinement\<close>
+
+fun expand :: "(nat, nat) com \<Rightarrow> ('v,'g,'r,'a) enuml \<Rightarrow> (('v,'g,'r,'a) auxop, ('v,'g,'r,'a) state) com"
+  where
+    "expand Nil l = Nil" |
+    "expand (Basic a) l = (case l ! tag a of (v,\<alpha>,f) \<Rightarrow> Basic (\<lfloor>v,\<alpha>,f\<rfloor>))" |
+    "expand (com.Seq c\<^sub>1 c\<^sub>2) l = com.Seq (expand c\<^sub>1 l) (expand c\<^sub>2 l)" |
+    "expand (Choice c\<^sub>1 c\<^sub>2) l = Choice (expand c\<^sub>1 l) (expand c\<^sub>2 l)" |
+    "expand (Loop c\<^sub>1) l = Loop (expand c\<^sub>1 l)" |
+    "expand (Parallel c\<^sub>1 c\<^sub>2) l = Parallel (expand c\<^sub>1 l) (expand c\<^sub>2 l)" |
+    "expand (Thread c\<^sub>1) l = Thread (expand c\<^sub>1 l)"
+
+fun expand_op 
+  where "expand_op (v,\<alpha>,f) = \<lfloor>v,\<alpha>,f\<rfloor>"
+
+fun expand_pairs :: "(nat \<times> ('g,'r) var fset) fset \<Rightarrow> ('v,'g,'r,'a) enuml \<Rightarrow> (('v,'g,'r,'a) opbasic \<times> ('g,'r) var set) set"
+  where
+    "expand_pairs p l = {(expand_op (l ! i), fset s) | i s. (i,s) \<in> fset p}"
+
+fun expand_point :: "('g,'r) point \<Rightarrow> ('v,'g,'r,'a) enuml \<Rightarrow> ('v,'g,'r,'a) SimAsm_Inter.point"
+  where
+    "expand_point p l = \<lparr> op = expand_op (l ! id p), 
+                          wrs = fset (wrs p), 
+                          rds = fset (rds p), 
+                          bar = bar p, 
+                          esc = fset (esc p),
+                          pairs = expand_pairs (pairs p) l \<rparr>"
+
+definition expand_points
+  where "expand_points P l = (\<lambda>s. expand_point s l) ` P"
 
 lemma [simp]:
-  "Sup (vars ` (all_points vs i :: ('a, 'b) point set) ) = vs"
-proof -
-  let ?f = "\<lambda>d w r b p. \<lparr>id = d, wrs = w, rds = r, bar = b, pairs = p\<rparr>"
-  have a: "(all_points vs i :: ('a, 'b) point set) = {?f d w r b p | d w r b p. w |\<subseteq>| vs \<and> r |\<subseteq>| vs \<and> d \<le> i \<and> nmax p \<le> i}"
-    unfolding all_points_def apply auto 
-    by (metis (full_types) old.unit.exhaust point.surjective)
+  "inst (\<lfloor>x1,x2,x3\<rfloor>) = x2"
+  by (auto simp: liftg_def)
 
-  have "(vars ` (all_points vs i :: ('a, 'b) point set)) = {j. j |\<subseteq>| vs}"
-    apply (auto simp: a)
-    apply (subgoal_tac "?f i x x True {||} \<in> all_points vs i")
-    unfolding a
-    apply force
-    by (auto simp: nmax_def)
-  moreover have "Sup {j. j |\<subseteq>| vs} = vs"
-    by (metis cSup_eq_maximum mem_Collect_eq order_refl)
-  ultimately show ?thesis by metis
-qed
-
-lemma all_points_nil:
-  "(all_points vs i :: ('a, 'b) point set) \<noteq> {}"
-proof -
-  have a: "\<lparr>id = 0, wrs = {||}, rds = {||}, bar = True, pairs = {||}\<rparr> \<in> all_points vs i"
-    by (auto simp: all_points_def nmax_def)
-  show ?thesis apply (rule ccontr) apply simp using a by blast
-qed
+lemma ldeps [simp]:
+  "set (ldeps e) = deps\<^sub>E e"
+proof (induct e)
+  case (Exp x1a x2a)
+  then show ?case apply ( simp add: fdeps_def)
+    by (smt Sup.SUP_cong fset_of_list.rep_eq set_list_bind)
+qed (auto simp: fdeps_def)
 
 lemma [simp]:
-  "Pmax (all_points vs i :: ('a, 'b) point set) = i"
-proof -
-  let ?f = "\<lambda>d w r b p. \<lparr>id = d, wrs = w, rds = r, bar = b, pairs = p\<rparr>"
-  have a: "(all_points vs i :: ('a, 'b) point set) = {?f d w r b p | d w r b p. w |\<subseteq>| vs \<and> r |\<subseteq>| vs \<and> d \<le> i \<and> nmax p \<le> i}"
-    unfolding all_points_def apply auto 
-    by (metis (full_types) old.unit.exhaust point.surjective)
-
-  have "id ` (all_points vs i  :: ('a, 'b) point set) = {j. j \<le> i}" unfolding a
-     apply auto 
-    by (smt fsubsetI mem_Collect_eq nmax_def point.simps(1) rev_image_eqI zero_order(1)) 
-  moreover have b: "Max {j. j \<le> i} = i"
-    by (metis Max_ge Max_in antisym emptyE finite_Collect_le_nat mem_Collect_eq order_refl)
-  ultimately have c: "Max (id ` (all_points vs i  :: ('a, 'b) point set)) = i" by simp
-
-  have "(nmax o pairs) ` (all_points vs i  :: ('a, 'b) point set) = {j. j \<le> i}" unfolding a
-    apply auto
-    apply (subgoal_tac "?f i vs vs True {|x|} \<in> all_points vs i")
-    apply (metis (no_types, lifting) a fMax.singleton finsert_not_fempty nmax_def point.select_convs(5) rev_image_eqI)
-    unfolding a by (auto simp: nmax_def)
-  hence d: "Max ((nmax o pairs) ` (all_points vs i  :: ('a, 'b) point set)) = i" using b by simp
-
-  have "(MAX p\<in>(all_points vs i :: ('a, 'b) point set). max (point.id p) (nmax (pairs p))) = i"
-    using Max_max[OF finite_all_points, of id "nmax o pairs" vs i]
-    unfolding c d by auto
-  thus "Pmax (all_points vs i :: ('a, 'b) point set) = i"
-    unfolding Pmax_def pmax_def using all_points_nil
-    by auto
-qed
-
-lemma sup_in:
-  assumes "finite P" "y \<in> P" "x |\<in>| f y"
-  shows "x |\<in>| Sup (f ` P)"
-proof -
-  have "x \<in> fset (f y)" using assms(3) by (meson notin_fset)
-  hence a: "x \<in> Sup ((fset o f) ` P)" using assms(2) by auto
-  have f: "finite ((\<Union>a\<in>P. fset (f a)))" using assms(1) by simp
-  hence "Sup ((fset o f) ` P) =  fset (Sup (f ` P))" 
-    unfolding Sup_fset_def apply auto
-    using Abs_fset_inverse f apply blast
-    using Abs_fset_inverse f by blast  
-  thus ?thesis using a notin_fset by metis
-qed
-
-lemma sup_in_l:
-  assumes "i < length l" "x |\<in>| f (l ! i)"
-  shows "x |\<in>| Sup (f ` set l)"
-  using assms sup_in[of "set l" "l ! i" x f] by auto
+  "fset (fdeps e) = deps\<^sub>E e"
+  by (simp add: fset_of_list.rep_eq fdeps_def)
 
 lemma [simp]:
-  "nmax (finsert a b) = max (a :: nat) (nmax b)"
-  unfolding nmax_def by auto
+  "fset (fdeps\<^sub>B e) = deps\<^sub>B e"
+proof (induct e)
+  case (Exp\<^sub>B x1a x2a)
+  then show ?case by (simp add: fset_of_list.rep_eq fdeps\<^sub>B_def set_list_bind)
+qed (auto simp: fdeps\<^sub>B_def)
 
-lemma proc1_all_points:
-  "finite P \<Longrightarrow> xa \<in> P \<Longrightarrow> tag x < length l \<Longrightarrow>
-          proc1 (tag x) (l ! tag x) xa
-          \<in> all_points
-              (varsL l |\<union>| Sup (vars ` P))
-              (max (length l) (Pmax P))"
-  unfolding proc1_def
-  apply (subgoal_tac "xa \<in> all_points
-              (varsL l |\<union>| Sup (vars ` P))
-              (max (length l) (Pmax P))")
-  apply (auto simp: all_points_def varsL_def)
-  apply (rule sup_in_l; blast)+
+lemma [simp]:
+  "fset (fwr a) = wr a"
+  by (cases a; auto)
 
-  apply (subgoal_tac "xb |\<in>| Sup (vars ` P)")
+lemma [simp]:
+  "fset (frd a) = rd a"
+  by (cases a; auto)
+
+lemma [simp]:
+  "fset (lfwr \<alpha>) = wr \<alpha> \<inter> locals"
+  by (cases \<alpha>; auto; case_tac x11; auto)
+
+lemma [simp]:
+  "hasGlobal\<^sub>e V = hasGlobal (fset V)"
+  unfolding hasGlobal\<^sub>e_def hasGlobal_def
+  by (meson notin_fset)
+
+lemma [simp]:
+  "((map (\<lambda>a. fst (snd a)) l' @ [x2]) ! length l') = x2"
+  by (metis length_map nth_append_length)
+
+lemma [simp]:
+  "(l @ [a,b]) ! Suc (length l) = b"
+  by (metis append_Cons append_Nil append_assoc length_append_singleton nth_append_length)
+
+lemma [intro]:
+  "a \<noteq> b \<Longrightarrow> fset a \<noteq> fset b"
+  by (simp add: fset_inject)
+
+lemma stren_exec:
+  "SimAsm_Inter.stren (expand_op \<alpha>) (expand_point p l) = expand_point (stren (fst (snd \<alpha>)) p) l"
+  by (cases \<alpha>; auto simp: stren_def SimAsm_Inter.stren_def)
+
+lemma wken_exec:
+  "l ! n = \<alpha> \<Longrightarrow> SimAsm_Inter.wken (expand_op \<alpha>) (expand_point p l) = expand_point (wken n (fst (snd \<alpha>)) p) l"
+  apply (clarsimp simp: wken_def SimAsm_Inter.wken_def)
+  apply (intro impI conjI)
+  apply (cases "l ! n"; clarsimp)
+  apply (cases "l ! n"; clarsimp)
+  apply (cases "l ! n"; clarsimp)
+  apply force
+  apply (cases "l ! n"; clarsimp)
+  apply (subgoal_tac "fset (fwr b |\<inter>| point.rds p) \<noteq> fset {||}")
   apply simp
-  apply (rule sup_in)
+  using fset_inject apply metis
+  apply (cases "l ! n"; clarsimp)
+  apply (cases "l ! n"; clarsimp)
+  apply force
+  apply (cases "l ! n"; clarsimp)
+  apply (subgoal_tac "fset (fwr b |\<inter>| point.rds p) = fset {||}")
+  apply fastforce
+  apply metis
+  apply (cases "l ! n"; clarsimp)
   apply blast
-  apply blast
-  apply blast
+  apply (cases "l ! n"; clarsimp)
+  apply (cases "l ! n"; clarsimp)
+  apply (cases "l ! n"; clarsimp)
+  by (smt Collect_cong expand_op.simps insert_Collect)
 
-  apply (subgoal_tac "xb |\<in>| Sup (vars ` P)")
-  apply simp
-  apply (rule sup_in)
-  apply blast
-  apply blast
-  apply blast
+lemma [intro]:
+  "x \<in> fset P \<Longrightarrow> x |\<in>| P"
+  by (meson notin_fset)
 
-  unfolding Pmax_def pmax_def
-  apply (simp add: Max_max)
-  apply (metis Max.bounded_iff empty_iff finite_imageI image_eqI max.cobounded1 max.coboundedI2)
-  apply (simp add: Max_max)
-  by (meson Max_ge empty_iff finite_imageI imageI le_max_iff_disj)
+lemma [intro]:
+  "x |\<in>| P \<Longrightarrow> x \<in> fset P"
+  by (meson notin_fset)
 
-lemma gen_all_points:
-  "tag x < length l \<Longrightarrow>
-          gen (tag x) (l ! tag x)
-          \<in> all_points
-              (varsL l |\<union>| Sup (vars ` P))
-              (max (length l) (Pmax P))"
-  unfolding gen_def all_points_def nmax_def varsL_def
-  apply auto
-  apply (rule sup_in_l; blast)+
-  done
-
-lemma rif_bound:
-  "finite P \<Longrightarrow> rif c l P \<subseteq> (all_points (varsL l |\<union>| Sup (vars ` P)) (max (length l) (Pmax P)) :: ('a, 'b) point set)"
-proof (induct c arbitrary: P)
-  case Nil
-  then show ?case using set_all_points_bound' by auto
-next
-  case (Basic x)
-  thus ?case
-    apply (auto simp: rif\<^sub>i_def proc\<^sub>i_def)
-    apply (rule gen_all_points; auto)
-    apply (rule proc1_all_points; auto)
-    using set_all_points_bound' by auto
-next
-  case (Seq c1 c2)
-  let ?V="(all_points(varsL l |\<union>| Sup (vars ` P)) (max (length l) (Pmax P)) :: ('a, 'b) point set)"
-  have f: "finite ?V" using finite_all_points by auto
-  show ?case using Seq(1)[OF f] Seq(2)[OF Seq(3)] by simp (meson dual_order.trans monoD mono_rif)
-next
-  case (Choice c1 c2)
-  then show ?case by auto
-next
-  case (Loop c)
-  show ?case
-    unfolding rif.simps
-    apply (rule lfp_lowerbound)
-    using Loop(1)[OF finite_all_points, of "(varsL l |\<union>| Sup (vars ` P))" "(max (length l) (Pmax P))"] set_all_points_bound'[OF Loop(2), of l]
-    by auto    
-next
-  case (Parallel c1 c2)
-  show ?case unfolding rif.simps using set_all_points_bound'[OF Parallel(3)] by auto
-next
-  case (Thread c)
-  show ?case unfolding rif.simps using set_all_points_bound'[OF Thread(2)] by auto
-qed
-
-subsection \<open>While Rule\<close>
-
-lemma rif_While:
-  fixes b c P l
-  assumes "finite (P :: ('a, 'b) point set)"
-  defines "f == (\<lambda>Y. (P \<union> rif c l Y))"
-  shows "rif (Loop c) l P = while (\<lambda>Y. f Y \<noteq> Y) f {}" (is "_ = ?r")
-proof -
-  let ?V = "all_points (varsL l |\<union>| Sup (vars ` P)) (max (length l) (Pmax P)) :: ('a, 'b) point set"
-  have "lfp f = ?r"
-  proof(rule lfp_while[where C = "?V"])
-    show "mono f" using f_def mono_union_rif by blast
-  next
-    fix Y assume a: "Y \<subseteq> ?V"
-    have f: "finite Y" using a finite_all_points finite_subset by blast 
-    have "P \<subseteq> ?V" using set_all_points_bound' assms(1) by blast
-    moreover have "SimAsm_Inter.rif c l Y \<subseteq> ?V"
-      using rif_bound[OF f, of c l] all_points_const[OF all_points_sub[OF a]] by force
-    ultimately show "f Y \<subseteq> ?V" unfolding f_def by blast
-  next
-    show "finite ?V" by (rule finite_all_points)
-  qed
-  thus ?thesis unfolding f_def rif.simps(3) by blast
-qed
-
-lemma rif_While_let: "finite X \<Longrightarrow> rif (Loop c) l X =
-  (let f = (\<lambda>Y. X \<union> rif c l Y) in while (\<lambda>Y. f Y \<noteq> Y) f {})"
-  by (simp add: rif_While)
-
-lemma rif_While_set: "rif (Loop c) l (set xs) =
-  (let f = (\<lambda>Y. set xs \<union> rif c l Y) in while (\<lambda>Y. f Y \<noteq> Y) f {})"
-  by (rule rif_While_let, simp)
-
-lemmas [code] = rif.simps(1,2,4,5,6,7) rif_While_set
-
-section \<open>fset Execution\<close>
-
-text \<open>List implementation of fset, similar to that of set\<close>
-
-code_datatype fset_of_list
-
-lemma fset_empty [code]:
-  "{||} = fset_of_list []"
+lemma ord_exec:
+  "ord (inst (expand_op \<alpha>)) (expand_point p l) = ord\<^sub>e (fst (snd \<alpha>)) p"
+  by (cases \<alpha>; case_tac b; auto split: var.splits)
+  
+lemma proc1_exec:
+  "l ! n = \<alpha> \<Longrightarrow> SimAsm_Inter.proc1 (expand_op \<alpha>) (expand_point p l) = expand_points (proc1 n (fst (snd \<alpha>)) p) l"
+  apply (simp only: expand_points_def wken_exec proc1_def SimAsm_Inter.proc1_def ord_exec stren_exec)
   by simp
 
-lemma fset_insert [code]:
-  "finsert a (fset_of_list x) = fset_of_list (List.insert a x)"
-  by (simp add: List.insert_def finsert_absorb fset_of_list_elem)
+lemma gen_exec:
+  "l ! n = \<alpha> \<Longrightarrow> SimAsm_Inter.gen (expand_op \<alpha>) = expand_point (gen n (fst (snd \<alpha>))) l"
+  by (cases "l ! n"; clarsimp)
 
-lemma fset_union [code]:
-  "fset_of_list a |\<union>| fset_of_list b = fset_of_list (List.union a b)"
-  by (metis fset_of_list.abs_eq fset_of_list_append set_append set_union)
+lemma rif\<^sub>i_exec:
+  "l ! n = \<alpha> \<Longrightarrow> SimAsm_Inter.rif\<^sub>i (expand_op \<alpha>) (expand_points P l) = expand_points (rif\<^sub>i n (fst (snd \<alpha>)) P) l"
+  apply (simp add: expand_points_def rif\<^sub>i_def SimAsm_Inter.rif\<^sub>i_def gen_exec proc1_exec del: expand_point.simps)
+  by blast
 
-lemma fset_inter [code]:
-  "A |\<inter>| fset_of_list xs = fset_of_list (List.filter (\<lambda>x. x |\<in>| A) xs)"
-  by auto
+lemma expand_points_union [simp]:
+  "expand_points (P \<union> Q) l = expand_points P l \<union> expand_points Q l"
+  by (auto simp: expand_points_def)
 
-lemma fset_remove [code]:
-  "fset_of_list xs |-| A = fset_of_list (List.filter (\<lambda>x. x |\<notin>| A) xs)"
-  by auto
+lemma expand_points_empty [simp]:
+  "expand_points {} l = {}"
+  by (auto simp: expand_points_def)
 
-lemma fset_hasGlobal [code]:
-  "hasGlobal (fset_of_list a) = hasGlobalL a"
-  by (induct a) (auto simp: hasGlobal_def; case_tac a1, auto)+
+lemma mono_rif\<^sub>i:
+  "mono (rif\<^sub>i n a)"
+  apply (rule monoI)
+  unfolding rif\<^sub>i_def by blast
 
-lemma fset_mem [code]:
-  "(x |\<in>| fset_of_list F) = (List.member F x)"
-  by (simp add: fset_of_list_elem member_def)
+lemma mono_rif:
+  "mono (rif c l)"
+proof (induct c)
+  case (Seq c1 c2)
+  then show ?case by (simp add: mono_def)
+next
+  case (Choice c1 c2)
+  then show ?case
+    by (smt Un_mono mono_def rif.simps(2))
+next
+  case (Loop c)
+  then show ?case 
+    by (smt Un_iff lfp_mono monoI subset_eq rif.simps(3))
+qed (simp add: monoI mono_rif\<^sub>i)+
 
-lemma fset_subset [code]:
-  "fset_of_list xs \<le> B \<longleftrightarrow> (\<forall>x\<in>set xs. x |\<in>| B)"
-  using fset_of_list.rep_eq notin_fset by fastforce
+lemma mono_union_rif':
+  "mono (\<lambda>Y. P \<union> rif c l Y)"
+  by (smt Un_mono monoD monoI mono_rif sup.idem sup.order_iff)
 
-declare fset_of_list_simps [code_post]
+lemma rif_exec:
+  "\<forall>\<beta> \<in> basics c. tag \<beta> < length l \<Longrightarrow>
+   SimAsm_Inter.rif (expand c l) (expand_points P l) = expand_points (rif c (map (fst o snd) l) P) l"
+proof (induct c arbitrary: P l)
+  case (Basic \<alpha>)
+  have e: "expand (Basic \<alpha>) l = Basic (expand_op (l ! tag \<alpha>))" by (cases \<alpha>; case_tac "l ! a"; auto)
+  have d: "map (\<lambda>a. fst (snd a)) l ! tag \<alpha> = fst (snd (l ! tag \<alpha>))" using Basic by simp
+  show ?case unfolding e by (simp add: d rif\<^sub>i_exec)
+next
+  case (Loop c)
+  let ?f="\<lambda>Y. expand_points P l \<union> SimAsm_Inter.rif (expand c l) Y"
+  let ?f'="\<lambda>Y. P \<union> rif c (map (\<lambda>a. fst (snd a)) l) Y"
 
-section \<open>Tactics\<close>
+  have r: "\<forall>P. SimAsm_Inter.rif (expand c l) (expand_points P l) = 
+               expand_points (rif c (map (fst \<circ> snd) l) P) l"
+    using Loop by fastforce
 
-text \<open>Tactic to match the executable analysis within more abstract properties\<close>
+  have r': "\<And>P. expand_points (rif c (map (\<lambda>a. fst (snd a)) l) P) l = 
+                SimAsm_Inter.rif (expand c l) (expand_points P l)"
+    using Loop unfolding o_def by fastforce
 
-attribute_setup get_conv = \<open>Args.term >> (fn t =>
-        Thm.rule_attribute [] (fn context => fn _ =>
-          (Code_Simp.dynamic_conv (Context.proof_of context) o Thm.cterm_of (Context.proof_of context)) t))\<close>
+  have "lfp ?f \<subseteq> expand_points (lfp ?f') l"
+  proof (induct rule: lfp_ordinal_induct[where ?f="?f"])
+    case mono
+    then show ?case by (simp add: mono_union_rif) 
+  next
+    case (step S)
+    hence "?f S \<subseteq> ?f (expand_points (lfp ?f') l)" 
+      using SimAsm_Inter.mono_rif monoD by blast      
+    also have "... \<subseteq> expand_points P l \<union> expand_points (rif c (map (\<lambda>a. fst (snd a)) l) (lfp ?f')) l"
+      using step by (simp add: o_def r)
+    also have "... \<subseteq> expand_points (P \<union> rif c (map (\<lambda>a. fst (snd a)) l) (lfp ?f')) l"
+      by auto
+    also have "... \<subseteq> expand_points (lfp ?f') l" 
+      by (metis lfp_unfold[OF mono_union_rif'] subset_refl)
+    finally show ?case  .
+  next
+    case (union M)
+    then show ?case by (cases "M = {}"; auto)
+  qed
 
-method rif_eval = 
-  (simp add: rif_checks_def rif_full_def del: rif.simps(1,2,4,5,6,7);
-   match conclusion in "checks l (rif c l' {}) R" for c and R 
-      and l :: "('a :: equal \<times>
-    ('b :: equal, 'c :: equal, 'd :: equal) op \<times>
-    (('b, ('c, 'd) SimAsm.var, 'e) state_rec_scheme
-     \<Rightarrow> 'e)) list"
-      and l' :: "('b :: equal, 'c  :: equal, 'd  :: equal) op list" \<Rightarrow>
-    \<open>match [[get_conv "rif c l' {}"]] in U: _ \<Rightarrow> \<open>subst U\<close>\<close>)
+  moreover have "expand_points (lfp ?f') l \<subseteq> lfp ?f"
+  proof (induct rule: lfp_ordinal_induct[where ?f="?f'"])
+    case mono
+    then show ?case by (simp add: mono_union_rif')
+  next
+    case (step S)
+    hence "?f (expand_points S l) \<subseteq>  ?f (lfp ?f)"
+      using SimAsm_Inter.mono_rif monoD by blast
+    also have "... \<subseteq> lfp ?f" using lfp_unfold[OF mono_union_rif] by blast
+    finally show ?case unfolding r' expand_points_union .
+  next
+    case (union M)
+    then show ?case by (cases "M = {}"; auto simp: expand_points_def)
+  qed
+
+  ultimately show ?case by (simp add: rif.simps(3))
+qed simp_all
+
+subsection \<open>Enumeration Properties\<close>
+
+text \<open>Enumeration only extends the list\<close>
+lemma enum_extends:
+  "enum c l\<^sub>1 = (r,l\<^sub>2) \<Longrightarrow> \<exists>l. l\<^sub>2 = l\<^sub>1 @ l"
+proof (induct c arbitrary: r l\<^sub>1 l\<^sub>2)
+  case (Seq c\<^sub>1 c\<^sub>2)
+  obtain r\<^sub>1 r\<^sub>2 l'' where r: "enum c\<^sub>2 l\<^sub>1 = (r\<^sub>2,l'')" "enum c\<^sub>1 l'' = (r\<^sub>1,l\<^sub>2)" "r = r\<^sub>1 ;; r\<^sub>2"
+    using Seq(3) by (cases "(lang.Seq c\<^sub>1 c\<^sub>2,l\<^sub>1)" rule: enum.cases) (auto split: prod.splits)
+  show ?case using Seq(1)[OF r(2)] Seq(2)[OF r(1)] Seq(3)  append.assoc by blast
+next
+  case (If b c\<^sub>1 c\<^sub>2)
+  obtain r\<^sub>1 r\<^sub>2 l\<^sub>3 l\<^sub>4 where r: 
+      "enum c\<^sub>2 l\<^sub>1 = (r\<^sub>2,l\<^sub>3)" 
+      "enum c\<^sub>1 l\<^sub>3 = (r\<^sub>1,l\<^sub>4)" 
+      "l\<^sub>2 = l\<^sub>4@[(UNIV,cmp b,state_rec.more),(UNIV,cmp (Neg b),state_rec.more)]"
+    using If(3) by (cases "(lang.If b c\<^sub>1 c\<^sub>2,l\<^sub>1)" rule: enum.cases) (auto split: prod.splits)
+  show ?case using If(1)[OF r(2)] If(2)[OF r(1)] If(3) r(3) by force
+next
+  case (While b x2 c)
+  obtain r\<^sub>1 l\<^sub>3 where r: 
+      "enum c l\<^sub>1 = (r\<^sub>1,l\<^sub>3)" 
+      "l\<^sub>2 = l\<^sub>3@[(UNIV,cmp b,state_rec.more),(UNIV,cmp (Neg b),state_rec.more)]"
+    using While(2) by (cases "(lang.While b x2 c,l\<^sub>1)" rule: enum.cases) (auto split: prod.splits)
+  show ?case using While(1)[OF r(1)] r(2) by auto
+next
+  case (DoWhile x1 c b)
+  obtain r\<^sub>1 l\<^sub>3 where r: 
+      "enum c l\<^sub>1 = (r\<^sub>1,l\<^sub>3)" 
+      "l\<^sub>2 = l\<^sub>3@[(UNIV,cmp b,state_rec.more),(UNIV,cmp (Neg b),state_rec.more)]"
+    using DoWhile(2) by (cases "(lang.DoWhile x1 c b,l\<^sub>1)" rule: enum.cases) (auto split: prod.splits)
+  then show ?case using DoWhile(1)[OF r(1)] by auto
+qed auto
+
+text \<open>Bounds on the instruction ids in the enumeration function\<close>
+lemma enum_basics_upper:
+  "enum c l' = (r,l) \<Longrightarrow> \<beta> \<in> basics r \<Longrightarrow> tag \<beta> < length l"
+  by (induct c arbitrary: r l l') (insert enum_extends, auto split: prod.splits; fastforce)+
+
+lemma expand_cong:
+  "\<forall>\<beta> \<in> basics c. l ! tag \<beta> = l' ! tag \<beta> \<Longrightarrow> expand c l = expand c l'"
+  by (induct c arbitrary: l l'; auto)
+
+lemma enum_expand_cong:
+  "enum c\<^sub>2 l\<^sub>1 = (r\<^sub>2, l\<^sub>2) \<Longrightarrow> enum c\<^sub>1 l\<^sub>2 = (r\<^sub>1, l\<^sub>3) \<Longrightarrow> expand r\<^sub>2 l\<^sub>2 = expand r\<^sub>2 l\<^sub>3"
+  by (metis (no_types, lifting) enum_basics_upper enum_extends expand_cong nth_append) 
+
+lemma concat_expand_cong:
+  "enum c\<^sub>1 l\<^sub>1 = (r\<^sub>1, l\<^sub>2) \<Longrightarrow> expand r\<^sub>1 l\<^sub>2 = expand r\<^sub>1 (l\<^sub>2 @ l)"
+  by (metis (no_types, lifting) enum_basics_upper expand_cong nth_append) 
+
+lemma liftl_lifg [intro!]:
+  "(liftl b) = (\<lfloor>UNIV,b,state_rec.more\<rfloor>)"
+  by (auto simp: liftg_def liftl_def)
+
+lemma enum_exec:
+  "enum c l' = (r,l) \<Longrightarrow> lift\<^sub>c c = expand r l"
+proof (induct c arbitrary: r l l')
+  case (Seq c1 c2)
+  thus ?case by (auto intro: enum_expand_cong split: prod.splits)
+next
+  case (If x1 c1 c2)
+  then show ?case
+    apply (auto split: prod.splits)
+    apply (rule concat_expand_cong; auto)
+    apply (rule expand_cong)
+    by (metis (no_types, lifting) append_assoc enum_basics_upper enum_extends nth_append)
+next
+  case (While x1 x2 c)
+  then show ?case by (auto intro: concat_expand_cong split: prod.splits)
+next
+  case (DoWhile x1 c x3)
+  then show ?case by (auto intro: concat_expand_cong split: prod.splits)
+qed auto
+
+subsection \<open>Link Abstract & Executable\<close>
+
+text \<open>Expand the abstract rif definition to an executable form\<close>
+lemma rif_executable:
+  "SimAsm_Inter.rif (lift\<^sub>c c) {} = (let (r,l) = enum c [] in expand_points (rif r (map (fst o snd) l) {}) l)"
+proof (unfold Let_def, case_tac "enum c []", clarsimp)
+  fix r l assume a: "enum c [] = (r,l)"
+  have "\<forall>\<beta>\<in>basics r. tag \<beta> < length l" using enum_basics_upper[OF a] by auto
+  hence "SimAsm_Inter.rif (expand r l) {} = expand_points (rif r (map (fst o snd) l) {}) l"
+    using rif_exec[where ?P="{}"] by auto
+  thus "SimAsm_Inter.rif (lift\<^sub>c c) {} = expand_points (rif r (map (fst \<circ> snd) l) {}) l"
+    using enum_exec a by force
+qed
 
 end
